chore: add iterator tests

src/Std/Data/DTreeMap/Iterator.lean
@@ -26,8 +26,8 @@ The iterator yields the elements of the map in order and then terminates.
 -/
 @[inline]
 public def iter {α : Type u} {β : α → Type v}
-    (cmp : α → α → Ordering := by exact compare) (m : DTreeMap α β cmp) :=
-  Raw.iter cmp ⟨m.inner⟩
+    {cmp : α → α → Ordering} (m : DTreeMap α β cmp) :=
+  @Raw.iter _ _ cmp ⟨m.inner⟩
 
 /--
 Returns a finite iterator over the keys of a dependent tree map.
@@ -41,9 +41,8 @@ The key and value types must live in the same universe.
 * `Productive` instance: always
 -/
 @[inline]
-public def keysIter {α : Type u} {β : α → Type u}
-    (cmp : α → α → Ordering := by exact compare) (m : DTreeMap α β cmp) :=
-  Raw.keysIter cmp ⟨m.inner⟩
+public def keysIter {α : Type u} {β : α → Type u} {cmp : α → α → Ordering} (m : DTreeMap α β cmp) :=
+  @Raw.keysIter _ _ cmp ⟨m.inner⟩
 
 /--
 Returns a finite iterator over the values of a tree map.
@@ -57,20 +56,20 @@ The key and value types must live in the same universe.
 * `Productive` instance: always
 -/
 @[inline]
-public def valuesIter {α : Type u} {β : Type u} (cmp : α → α → Ordering := by exact compare)
+public def valuesIter {α : Type u} {β : Type u} {cmp : α → α → Ordering}
     (m : DTreeMap α (fun _ => β) cmp) :=
-  Raw.valuesIter cmp ⟨m.inner⟩
+  @Raw.valuesIter _ _ cmp  ⟨m.inner⟩
 
 @[simp]
 public theorem iter_toList {cmp : α → α → Ordering} (m : DTreeMap α β cmp) :
-    (m.iter cmp).toList = m.toList := Raw.iter_toList ⟨m.inner⟩
+    m.iter.toList = m.toList := Raw.iter_toList ⟨m.inner⟩
 
 @[simp]
-public theorem keysIter_toList {α β} {cmp : α → α → Ordering} (m : DTreeMap α β cmp) :
-    (m.keysIter cmp).toList = m.keys := Raw.keysIter_toList ⟨m.inner⟩
+public theorem keysIter_toList {cmp : α → α → Ordering} (m : DTreeMap α β cmp) :
+    m.keysIter.toList = m.keys := Raw.keysIter_toList ⟨m.inner⟩
 
 @[simp]
-public theorem valuesIter_toList {α β} {cmp : α → α → Ordering} (m : DTreeMap α (fun _ => β) cmp) :
-    (m.valuesIter cmp).toList = m.values := Raw.valuesIter_toList ⟨m.inner⟩
+public theorem valuesIter_toList {cmp : α → α → Ordering} (m : DTreeMap α (fun _ => β) cmp) :
+    m.valuesIter.toList = m.values := Raw.valuesIter_toList ⟨m.inner⟩
 
 end Std.DTreeMap
