src/Std/Data/TreeMap/Iterator.lean
@@ -27,8 +27,8 @@ The iterator yields the elements of the map in order and then terminates.
 -/
 @[inline]
 public def iter {α : Type u} {β : Type v}
-    (cmp : α → α → Ordering := by exact compare) (m : TreeMap α β cmp) :=
-  ((m.inner.iter cmp).map fun e => (e.1, e.2) : Iter (α × β))
+    {cmp : α → α → Ordering} (m : TreeMap α β cmp) :=
+  (m.inner.iter.map fun e => (e.1, e.2) : Iter (α × β))
 
 /--
 Returns a finite iterator over the keys of a tree map.
@@ -43,8 +43,8 @@ The key and value types must live in the same universe.
 -/
 @[inline]
 public def keysIter {α : Type u} {β : Type u}
-    (cmp : α → α → Ordering := by exact compare) (m : TreeMap α β cmp) :=
-  m.inner.keysIter cmp
+    {cmp : α → α → Ordering} (m : TreeMap α β cmp) :=
+  m.inner.keysIter
 
 /--
 Returns a finite iterator over the values of a tree map.
@@ -58,13 +58,13 @@ The key and value types must live in the same universe.
 * `Productive` instance: always
 -/
 @[inline]
-public def valuesIter {α : Type u} {β : Type u} (cmp : α → α → Ordering := by exact compare)
+public def valuesIter {α : Type u} {β : Type u} {cmp : α → α → Ordering}
     (m : TreeMap α β cmp) :=
-  m.inner.valuesIter cmp
+  m.inner.valuesIter
 
 @[simp]
 public theorem iter_toList {cmp : α → α → Ordering} (m : TreeMap α β cmp) :
-    (m.iter cmp).toList = m.toList := by
+    m.iter.toList = m.toList := by
   simp only [iter, Iter.toList_map, DTreeMap.iter_toList, DTreeMap.toList,
     DTreeMap.Internal.Impl.toList_eq_toListModel, toList, DTreeMap.Const.toList,
     DTreeMap.Internal.Impl.Const.toList_eq_toListModel_map]
@@ -72,12 +72,12 @@ public theorem iter_toList {cmp : α → α → Ordering} (m : TreeMap α β cmp
 
 @[simp]
 public theorem keysIter_toList {α β} {cmp : α → α → Ordering} (m : TreeMap α β cmp) :
-    (m.keysIter cmp).toList = m.keys :=
+    m.keysIter.toList = m.keys :=
   m.inner.keysIter_toList
 
 @[simp]
 public theorem valuesIter_toList {α β} {cmp : α → α → Ordering} (m : TreeMap α β cmp) :
-    (m.valuesIter cmp).toList = m.values :=
+    m.valuesIter.toList = m.values :=
   m.inner.valuesIter_toList
 
 end Std.TreeMap
